theories/Syntax/Patterns.v
@@ -22,6 +22,8 @@
 (* SOFTWARE, EVEN IF ADVISED OF THE POSSIBILITY OF SUCH DAMAGE.               *)
 (******************************************************************************)
 
+From Coq Require Import Init.Logic.
+
 From Katamaran Require Import
      Prelude
      Context
@@ -228,6 +230,18 @@ Module Type PatternsOn (Import TY : Types).
       (* | pat_union U p          => fun '(existT K pc) => PatternCaseCtx pc *)
       end%ctx.
 
+    Definition isSinglePattern {σ} (p : Pattern σ) : bool :=
+      match p with
+      | pat_var x              => true
+      | pat_bool               => false
+      (* | pat_list σ x y         => false *)
+      | pat_pair x y           => true
+      (* | pat_sum σ τ x y        => false *)
+      | pat_unit               => true
+      (* | pat_enum E             => false *)
+      | pat_bvec_split m n x y => true
+      end.
+
     Definition MatchResult {σ} (pat : Pattern σ) : Type :=
       { c : PatternCase pat & NamedEnv Val (PatternCaseCtx c) }.
     #[global] Arguments MatchResult {σ} !pat /.
@@ -366,8 +380,6 @@ Module Type PatternsOn (Import TY : Types).
       pattern_match_val pat (pattern_match_val_reverse pat pc δpc) = (existT pc δpc).
     Proof. apply (pattern_match_val_inverse_right' pat (existT pc δpc)). Qed.
 
-
-    (* TODO: This lemma is wrong, because currently NonSyncVal for ty.unit is possible, but when reversing a unit, we know it's no NonSyncVal. *)
     Lemma pattern_match_val_inverse_left {σ} (pat : Pattern σ) :
       forall v : Val σ,
         pattern_match_val_reverse' pat (pattern_match_val pat v) = v.
@@ -397,6 +409,293 @@ Module Type PatternsOn (Import TY : Types).
       (*     (pattern_match_val_reverse' _ (existT pc vs)). *)
       (*   now rewrite <- Heq, H. *)
     Qed.
+
+
+    Definition MatchResultRel {σ} (pat : Pattern σ) : Type :=
+      { c : PatternCase pat & NamedEnv RelVal (PatternCaseCtx c) }.
+    #[global] Arguments MatchResultRel {σ} !pat /.
+
+    Definition match_result_rel_to_nonsyncval {σ} {pat : Pattern σ} (mr : @MatchResultRel σ pat) :=
+      @existT (PatternCase pat) (fun (ctx : PatternCase pat) => NamedEnv RelVal (PatternCaseCtx ctx))
+        (projT1 mr) (ty.namedEnvRel_to_nonsyncval (projT2 mr)).
+
+
+    Definition pattern_match_relval {σ} (p : Pattern σ) : RelVal σ -> MatchResultRel p :=
+      match p in Pattern σ return RelVal σ -> MatchResultRel p with
+      | pat_var x =>
+          fun v => existT tt [env].[x∷_ ↦ v]
+      | pat_bool       =>
+          fun b => existT (ty.projLeft b) [env]
+      (* | pat_list σ x y => *)
+      (*     fun v : Val (ty.list σ) => *)
+      (*       match v with *)
+      (*       | nil       => existT true [env] *)
+      (*       | cons v vs => existT false [env].[x∷σ ↦ v].[y∷ty.list σ ↦ vs] *)
+      (*       end *)
+      | pat_pair x y =>
+          fun v => match ty.relValPairIsPairRelVal v with
+                   | (a , b) => existT tt [env].[x∷_ ↦ a].[y∷_ ↦ b]
+                   end
+      (* | pat_sum σ τ x y => *)
+      (*     fun v => *)
+      (*       match v with *)
+      (*       | inl a => existT true [env].[x∷σ ↦ a] *)
+      (*       | inr b => existT false [env].[y∷τ ↦ b] *)
+      (*       end *)
+      | pat_unit =>
+          fun _ => existT tt [env]
+      (* | pat_enum E => *)
+      (*     fun v : enumt E => existT v [env] *)
+      | pat_bvec_split m n x y =>
+          fun v =>
+            match v with
+            | ty.SyncVal _ v' =>
+                match bv.appView m n v' with
+                | bv.isapp xs ys =>
+                    existT tt [env].[x∷ty.bvec m ↦ ty.SyncVal (ty.bvec _) xs].[y∷ty.bvec n ↦ ty.SyncVal (ty.bvec _) ys]
+                end
+            | ty.NonSyncVal _ v1 v2 =>
+                match bv.appView m n v1 , bv.appView m n v2 with
+                | bv.isapp xs1 ys1 , bv.isapp xs2 ys2 =>
+                    existT tt [env].[x∷ty.bvec m ↦ ty.NonSyncVal (ty.bvec _) xs1 xs2].[y∷ty.bvec n ↦ ty.NonSyncVal (ty.bvec _) ys1 ys2]
+                end
+            end
+              (* | pat_bvec_exhaustive m => *)
+              (*     fun v => existT v [env] *)
+              (* | pat_tuple p => *)
+              (*     fun v => existT tt (tuple_pattern_match_val p v) *)
+              (* | pat_record R Δ p => *)
+              (*     fun v => existT tt (record_pattern_match_val p v) *)
+              (* | pat_union U p => *)
+              (*     fun v => *)
+              (*       let (K, u)    := unionv_unfold U v in *)
+              (*       let (pc, δpc) := pattern_match_val (p K) u in *)
+              (*       (existT (existT K pc) δpc) *)
+      end.
+    #[global] Arguments pattern_match_relval {σ} !p v.
+
+
+    Definition pattern_match_relval_reverse {σ} (p : Pattern σ) :
+      forall (c : PatternCase p), NamedEnv RelVal (PatternCaseCtx c) -> RelVal σ :=
+      match p with
+      | pat_var x      => fun _ vs => env.head vs
+      | pat_bool       => fun b _ => ty.SyncVal ty.bool b
+      (* | pat_list σ x y => *)
+      (*     fun b => *)
+      (*       match b with *)
+      (*       | true  => fun _ => nil *)
+      (*       | false => fun Eht => *)
+      (*                    let (Eh,t) := env.view Eht in *)
+      (*                    let (E,h)  := env.view Eh in *)
+      (*                    cons h t *)
+      (*       end *)
+      | pat_pair x y =>
+          fun _ Exy =>
+            let (Ex,vy) := env.view Exy in
+            let (E,vx)  := env.view Ex in
+            ty.pairRelValIsRelValPair (vx,vy)
+      (* | pat_sum σ τ x y => *)
+      (*     fun b => *)
+      (*       match b with *)
+      (*       | true  => fun vs => inl (env.head vs) *)
+      (*       | false => fun vs => inr (env.head vs) *)
+      (*       end *)
+      | pat_unit =>
+          fun _ _ => ty.SyncVal ty.unit tt
+      (* | pat_enum E => *)
+      (*     fun v _ => v *)
+      | pat_bvec_split m n x y =>
+          fun _ Exy =>
+            let (Ex,vy) := env.view Exy in
+            let (E,vx)  := env.view Ex in
+            @ty.liftBinOp _ _ (ty.bvec m) (ty.bvec n) (ty.bvec (m + n)) bv.app vx vy
+      (* | pat_bvec_exhaustive m => *)
+      (*     fun v _ => v *)
+      (* | pat_tuple p => *)
+      (*     fun _ vs => envrec.of_env (tuple_pattern_match_env_reverse p vs) *)
+      (* | pat_record R Δ p => *)
+      (*     fun _ vs => recordv_fold R (record_pattern_match_env_reverse p vs) *)
+      (* | pat_union U p => *)
+      (*     fun '(existT K pc) δpc => *)
+      (*       unionv_fold U (existT K (pattern_match_val_reverse (p K) pc δpc)) *)
+      end.
+
+    Definition pat_relval_reverse_is_always_syncval {σ} (p : Pattern σ) : bool :=
+      match p with
+      | pat_bool => true
+      | pat_unit => true
+      | _ => false
+      end.
+
+    (* A curried version of the above. *)
+    Definition pattern_match_relval_reverse' {σ} (p : Pattern σ) :
+      MatchResultRel p -> RelVal σ :=
+      fun c => pattern_match_relval_reverse p (projT1 c) (projT2 c).
+
+
+    (* This does not seem to be true, because a pair (SyncVal, NonSyncVal), becomes (NonSyncVal, NonSyncVal) *)
+    (*   Lemma pattern_match_relval_inverse_right' {σ} (p : Pattern σ) : *)
+    (*   forall (r : MatchResultRel p), *)
+    (*     pattern_match_relval p (pattern_match_relval_reverse' p r) = r. *)
+    (* Proof. *)
+    (*   induction p; cbn; intros [pc vs]; try progress cbn. *)
+    (*   - destruct pc; now env.destroy vs. *)
+    (*   - env.destroy vs. reflexivity. *)
+    (*   - destruct pc. env.destroy vs. destruct v0; destruct v; cbn; try reflexivity. *)
+    (*   - destruct pc; now env.destroy vs. *)
+    (*   (* - destruct pc; now env.destroy vs. *) *)
+    (*   (* - destruct pc; now env.destroy vs. *) *)
+    (*   (* - now env.destroy vs. *) *)
+    (*   - destruct pc; env.destroy vs. *)
+    (*     now rewrite bv.appView_app. *)
+    (*   (* - now env.destroy vs. *) *)
+    (*   (* - destruct pc. *) *)
+    (*   (*   unfold tuple_pattern_match_val. *) *)
+    (*   (*   rewrite envrec.to_of_env. *) *)
+    (*   (*   now rewrite tuple_pattern_match_env_inverse_right. *) *)
+    (*   (* - destruct pc. *) *)
+    (*   (*   unfold record_pattern_match_val. *) *)
+    (*   (*   rewrite recordv_unfold_fold. *) *)
+    (*   (*   now rewrite record_pattern_match_env_inverse_right. *) *)
+    (*   (* - destruct pc as [K pc]. *) *)
+    (*   (*   rewrite unionv_unfold_fold. *) *)
+    (*   (*   change (pattern_match_val_reverse _ ?pc ?vs) with *) *)
+    (*   (*     (pattern_match_val_reverse' _ (existT pc vs)). *) *)
+    (*   (*   now rewrite H. *) *)
+    (* Qed. *)
+
+    Lemma pattern_match_syncval_inverse_right {σ} (pat : Pattern σ)
+      (pc : PatternCase pat) (δpc : NamedEnv Val (PatternCaseCtx pc)) :
+      pattern_match_relval pat (pattern_match_relval_reverse pat pc (ty.mapSyncValNamedEnv δpc)) = (existT pc (ty.mapSyncValNamedEnv δpc)).
+    Proof.
+      induction pat; cbn; try progress cbn.
+      - destruct pc. cbn in δpc. now env.destroy δpc.
+      - env.destroy δpc. cbn in δpc. env.destroy δpc. reflexivity.
+      - destruct pc. cbn in δpc. env.destroy δpc. cbn. reflexivity.
+      - destruct pc; cbn in δpc; now env.destroy δpc.
+      (* - destruct pc; now env.destroy vs. *)
+      (* - destruct pc; now env.destroy vs. *)
+      (* - now env.destroy vs. *)
+      - destruct pc; env.destroy δpc. destruct (ty.mapSyncValNamedEnv δpc); env.destroy δpc;
+        cbn;
+        now rewrite bv.appView_app.
+      (* - now env.destroy vs. *)
+      (* - destruct pc. *)
+      (*   unfold tuple_pattern_match_val. *)
+      (*   rewrite envrec.to_of_env. *)
+      (*   now rewrite tuple_pattern_match_env_inverse_right. *)
+      (* - destruct pc. *)
+      (*   unfold record_pattern_match_val. *)
+      (*   rewrite recordv_unfold_fold. *)
+      (*   now rewrite record_pattern_match_env_inverse_right. *)
+      (* - destruct pc as [K pc]. *)
+      (*   rewrite unionv_unfold_fold. *)
+      (*   change (pattern_match_val_reverse _ ?pc ?vs) with *)
+      (*     (pattern_match_val_reverse' _ (existT pc vs)). *)
+      (*   now rewrite H. *)
+    Qed.
+
+
+    (* TODO: This is currently not correct. *)
+    Lemma pmrevNonSyncImpliesAllNonSync {σ pat v1 v2} : ty.allNonSync (projT2 (pattern_match_relval pat (ty.NonSyncVal σ v1 v2))).
+    Proof.
+      destruct pat; cbn; try tauto.
+      - destruct v1. destruct v2. cbn. tauto.
+      - destruct (bv.appView m n v1). destruct (bv.appView m n v2). cbn. tauto.
+    Qed.
+
+        Lemma pattern_match_nonsyncval_inverse_right {σ} (pat : Pattern σ)
+      (pc : PatternCase pat) (δpc : NamedEnv RelVal (PatternCaseCtx pc)) :
+          match_result_rel_to_nonsyncval (pattern_match_relval pat (pattern_match_relval_reverse pat pc δpc)) = match_result_rel_to_nonsyncval (existT pc δpc).
+    Proof.
+      induction pat; cbn; try progress cbn.
+      - destruct pc. cbn in δpc. now env.destroy δpc.
+      - env.destroy δpc. cbn in δpc. env.destroy δpc. reflexivity.
+      - destruct pc. cbn in δpc. env.destroy δpc. destruct v0; destruct v; cbn; reflexivity.
+      - destruct pc; cbn in δpc; now env.destroy δpc.
+      (* - destruct pc; now env.destroy vs. *)
+      (* - destruct pc; now env.destroy vs. *)
+      (* - now env.destroy vs. *)
+      - destruct pc; env.destroy δpc. destruct (env.view δpc). destruct (env.view E). env.destroy E. cbn.
+        destruct v0; destruct v; cbn; rewrite bv.appView_app; cbn; try reflexivity;
+          rewrite bv.appView_app; reflexivity.
+    Qed.
+
+    (* Lemma pattern_match_relval_inverse_left {σ} (pat : Pattern σ) : *)
+    (*   forall v : RelVal σ, *)
+    (*     pattern_match_relval_reverse' pat (pattern_match_relval pat v) = v. *)
+    (* Proof. *)
+    (*   induction pat; cbn; intros v; try progress cbn. *)
+    (*   - reflexivity. *)
+    (*   - reflexivity. *)
+    (*   - destruct v; reflexivity. *)
+    (*   (* - destruct v; destruct v; cbn; try reflexivity. *) *)
+    (*   (*   destruct v0; cbn; reflexivity. *) *)
+    (*   - destruct v; reflexivity. *)
+    (*   (* - destruct v. reflexivity. *) *)
+    (*   (* - reflexivity. *) *)
+    (*   - destruct bv.appView; reflexivity. *)
+    (*   (* - reflexivity. *) *)
+    (*   (* - unfold tuple_pattern_match_val. *) *)
+    (*   (*   rewrite tuple_pattern_match_env_inverse_left. *) *)
+    (*   (*   now rewrite envrec.of_to_env. *) *)
+    (*   (* - unfold record_pattern_match_val. *) *)
+    (*   (*   rewrite record_pattern_match_env_inverse_left. *) *)
+    (*   (*   now rewrite recordv_fold_unfold. *) *)
+    (*   (* - destruct unionv_unfold as [K v'] eqn:Heq. *) *)
+    (*   (*   apply (f_equal (unionv_fold U)) in Heq. *) *)
+    (*   (*   rewrite unionv_fold_unfold in Heq. subst. *) *)
+    (*   (*   destruct pattern_match_val eqn:Heq; cbn. *) *)
+    (*   (*   change (pattern_match_val_reverse _ ?pc ?vs) with *) *)
+    (*   (*     (pattern_match_val_reverse' _ (existT pc vs)). *) *)
+    (*   (*   now rewrite <- Heq, H. *) *)
+    (* Qed. *)
+
+        Lemma pattern_match_syncval_inverse_left {σ} (pat : Pattern σ) :
+      forall v : Val σ,
+        pattern_match_relval_reverse' pat (pattern_match_relval pat (ty.SyncVal σ v)) = (ty.SyncVal σ v).
+    Proof.
+      induction pat; cbn; intros v; try progress cbn.
+      - reflexivity.
+      - reflexivity.
+      - destruct v; reflexivity.
+      (* - destruct v; destruct v; cbn; try reflexivity. *)
+      (*   destruct v0; cbn; reflexivity. *)
+      - destruct v; reflexivity.
+      (* - destruct v. reflexivity. *)
+      (* - reflexivity. *)
+      - destruct bv.appView; reflexivity.
+      (* - reflexivity. *)
+      (* - unfold tuple_pattern_match_val. *)
+      (*   rewrite tuple_pattern_match_env_inverse_left. *)
+      (*   now rewrite envrec.of_to_env. *)
+      (* - unfold record_pattern_match_val. *)
+      (*   rewrite record_pattern_match_env_inverse_left. *)
+      (*   now rewrite recordv_fold_unfold. *)
+      (* - destruct unionv_unfold as [K v'] eqn:Heq. *)
+      (*   apply (f_equal (unionv_fold U)) in Heq. *)
+      (*   rewrite unionv_fold_unfold in Heq. subst. *)
+      (*   destruct pattern_match_val eqn:Heq; cbn. *)
+      (*   change (pattern_match_val_reverse _ ?pc ?vs) with *)
+      (*     (pattern_match_val_reverse' _ (existT pc vs)). *)
+      (*   now rewrite <- Heq, H. *)
+    Qed.
+
+
+            Lemma pattern_match_nonsyncval_inverse_left {σ} (pat : Pattern σ) :
+      forall v1 v2 : Val σ,
+        isSinglePattern pat = true ->
+        pat_relval_reverse_is_always_syncval pat = false ->
+        (pattern_match_relval_reverse' pat (pattern_match_relval pat (ty.NonSyncVal σ v1 v2)) = ty.NonSyncVal σ v1 v2).
+    Proof.
+      induction pat; cbn; intros v1 v2 eq1 eq2; try progress cbn.
+      - reflexivity.
+      - congruence.
+      - destruct v1; destruct v2; reflexivity.
+      - congruence.
+      - destruct bv.appView. destruct bv.appView. reflexivity.
+    Qed.
+
 
     (* The intendend use case of the above definitions is in the declaration of
        inductive types for AST that represent pattern matches. This will
